Use the new add_relsimp facilities in simpLib to implement the system provided by reductionEval, and to simplify the proofs in chap2Script. While I'm at it, add definitions and characterising theorems about combinators B, C, and Y in chap2Theory.

examples/lambda/barendregt/chap2Script.sml
@@ -169,6 +169,10 @@ val lemma2_12 = store_thm( (* p. 19 *)
     PROVE_TAC [lam_eq_rules]
   ]);
 
+val lameq_sub_cong = save_thm(
+  "lameq_sub_cong", 
+  REWRITE_RULE [GSYM AND_IMP_INTRO] (last (CONJUNCTS lemma2_12)));
+
 val lemma2_13 = store_thm( (* p.20 *)
   "lemma2_13",
   ``!c n n'. ctxt c ==> (n == n') ==> (c n == c n')``,
@@ -241,14 +245,24 @@ val S_def =
     Define`S = LAM "x" (LAM "y" (LAM "z"
                                      ((VAR "x" @@ VAR "z") @@
                                       (VAR "y" @@ VAR "z"))))`;
+val FV_S = Store_thm(
+  "FV_S", 
+  ``FV S = {}``,
+  SRW_TAC [][S_def, EXTENSION] THEN METIS_TAC []);
+
 val K_def = Define`K = LAM "x" (LAM "y" (VAR "x"))`;
+val FV_K = Store_thm(
+  "FV_K", 
+  ``FV K = {}``, 
+  SRW_TAC [][K_def, EXTENSION])
+
 val I_def = Define`I = LAM "x" (VAR "x")`;
+val FV_I = Store_thm("FV_I", ``FV I = {}``, SRW_TAC [][I_def]);
 
 val Omega_def =
     Define`Omega = (LAM "x" (VAR "x" @@ VAR "x")) @@
                      (LAM "x" (VAR "x" @@ VAR "x"))`
 val _ = Unicode.unicode_version {tmnm = "Omega", u = UnicodeChars.Omega}
-
 val FV_Omega = Store_thm(
   "FV_Omega",
   ``FV Omega = {}``,
@@ -270,66 +284,78 @@ val lameq_asmlam = store_thm(
   ``!M N. M == N ==> asmlam eqns M N``,
   HO_MATCH_MP_TAC lam_eq_indn THEN METIS_TAC [asmlam_rules]);
 
+fun betafy ss = 
+    simpLib.add_relsimp {refl = GEN_ALL lameq_refl, 
+                         trans = List.nth(CONJUNCTS lam_eq_rules, 3), 
+                         weakenings = [lameq_weaken_cong], 
+                         subsets = [], 
+                         rewrs = [hd (CONJUNCTS lam_eq_rules)]} ss ++ 
+    simpLib.SSFRAG {rewrs = [], 
+                    ac = [],  convs = [],
+                    congs = [lameq_app_cong, 
+                             SPEC_ALL (last (CONJUNCTS lam_eq_rules)),
+                             lameq_sub_cong],
+                    dprocs = [], filter = NONE, name = NONE}
+
 val lameq_S = store_thm(
   "lameq_S",
   ``S @@ A @@ B @@ C == (A @@ C) @@ (B @@ C)``,
-  Q_TAC (NEW_TAC "y") `{"x"; "y"; "z"} UNION FV A UNION FV B UNION FV C` THEN
-  Q_TAC (NEW_TAC "z")
-        `{y; "x"; "y"; "z"} UNION FV A UNION FV B UNION FV C` THEN
-  Q.ABBREV_TAC `S1 = LAM y (LAM z ((A @@ VAR z) @@ (VAR y @@ VAR z)))` THEN
-  `S @@ A == S1`
-     by (Q_TAC SUFF_TAC `?x M. (S = LAM x M) /\ (S1 = [A/x]M)` THEN1
-           PROVE_TAC [lam_eq_rules] THEN
-         Q.EXISTS_TAC `"x"` THEN SRW_TAC [][S_def] THEN
-        `LAM "y" (LAM "z" ((VAR "x" @@ VAR "z") @@ (VAR "y" @@ VAR "z"))) =
-         LAM y (LAM z ((VAR "x" @@ VAR z) @@ (VAR y @@ VAR z)))` by
-           ASM_SIMP_TAC (srw_ss()) [SUB_THM, LAM_eq_thm] THEN
-        POP_ASSUM SUBST_ALL_TAC THEN
-        ASM_SIMP_TAC (srw_ss()) [SUB_THM]) THEN
-  `S @@ A @@ B @@ C == S1 @@ B @@ C` by PROVE_TAC [lam_eq_rules] THEN
-  Q_TAC SUFF_TAC `S1 @@ B @@ C == A @@ C @@ (B @@ C)` THEN1
-    PROVE_TAC [lam_eq_rules] THEN
-  Q.ABBREV_TAC `S2 = LAM z (A @@ VAR z @@ (B @@ VAR z))` THEN
-  `S1 @@ B == S2` by
-     (Q_TAC SUFF_TAC `?M. (S1 = LAM y M) /\ (S2 = [B/y]M)` THEN1
-        PROVE_TAC [lam_eq_rules] THEN
-      NTAC 2 (FIRST_X_ASSUM (SUBST_ALL_TAC o SYM)) THEN
-      ASM_SIMP_TAC (srw_ss()) [lemma14b]) THEN 
-  Q_TAC SUFF_TAC `S2 @@ C == A @@ C @@ (B @@ C)` THEN1
-      PROVE_TAC [lam_eq_rules] THEN
-  Q_TAC SUFF_TAC `?M. (S2 = LAM z M) /\ (A @@ C @@ (B @@ C) = [C/z]M)` THEN1
-      PROVE_TAC [lam_eq_rules] THEN
-  NTAC 2 (FIRST_X_ASSUM (SUBST_ALL_TAC o SYM)) THEN
-  ASM_SIMP_TAC (srw_ss()) [lemma14b]);
+  SIMP_TAC (srw_ss()) [S_def] THEN FRESH_TAC THEN 
+  ASM_SIMP_TAC (betafy (srw_ss())) [lemma14b]);
 
 val lameq_K = store_thm(
   "lameq_K",
   ``K @@ A @@ B == A``,
-  Q_TAC (NEW_TAC "x") `{"x"; "y"} UNION FV A UNION FV B` THEN
-  Q_TAC (NEW_TAC "y") `{x; "x"; "y"} UNION FV A UNION FV B` THEN
-  `K = LAM x (LAM y (VAR x))`
-     by SRW_TAC [][K_def, LAM_eq_thm, basic_swapTheory.swapstr_def,
-                   stringTheory.CHR_11] THEN
-  POP_ASSUM SUBST_ALL_TAC THEN
-  Q_TAC SUFF_TAC
-    `LAM x (LAM y (VAR x)) @@ A @@ B == (LAM y A) @@ B
-        /\
-     LAM y A @@ B == A`
-    THEN1 PROVE_TAC [lam_eq_rules] THEN
-  CONJ_TAC THENL [
-    Q_TAC SUFF_TAC `[A/x](LAM y (VAR x)) = LAM y A` THEN1
-      PROVE_TAC [lam_eq_rules] THEN
-    ASM_SIMP_TAC std_ss [SUB_THM],
-    Q_TAC SUFF_TAC `[B/y]A = A` THEN1 PROVE_TAC [lam_eq_rules] THEN
-    ASM_SIMP_TAC std_ss [lemma14b]
-  ]);
+  REWRITE_TAC [K_def] THEN FRESH_TAC THEN 
+  ASM_SIMP_TAC (betafy (srw_ss())) [lemma14b]);
 
 val lameq_I = store_thm(
   "lameq_I",
   ``I @@ A == A``,
   PROVE_TAC [lam_eq_rules, I_def, SUB_THM]);
 
-val FV_I = Store_thm("FV_I", ``FV I = {}``, SRW_TAC [][I_def]);
+val B_def = Define`B = S @@ (K @@ S) @@ K`;
+val FV_B = Store_thm(
+  "FV_B",
+  ``FV B = {}``,
+  SRW_TAC [][B_def]);
+
+val lameq_B = store_thm(
+  "lameq_B",
+  ``B @@ f @@ g @@ x == f @@ (g @@ x)``,
+  SIMP_TAC (betafy (srw_ss())) [lameq_S, lameq_K, B_def]);
+
+val C_def = Define`
+  C = S @@ (B @@ B @@ S) @@ (K @@ K)
+`;
+val FV_C = Store_thm(
+  "FV_C",
+  ``FV C = {}``,
+  SRW_TAC [][C_def]); 
+
+val lameq_C = store_thm(
+  "lameq_C",
+  ``C @@ f @@ x @@ y == f @@ y @@ x``,
+  SIMP_TAC (betafy (srw_ss())) [C_def, lameq_S, lameq_K, lameq_B]);
+
+val Y_def = Define`
+  Y = S @@ (C @@ B @@ (S @@ I @@ I)) @@ (C @@ B @@ (S @@ I @@ I))
+`;
+val FV_Y = Store_thm("FV_Y", ``FV Y = {}``, SRW_TAC [][Y_def]);
+
+val Yf1 = prove(
+  ``B @@ f @@ (S @@ I @@ I) @@ (B @@ f @@ (S @@ I @@ I)) == Y @@ f``,
+  SIMP_TAC (betafy(srw_ss())) [lameq_S, Y_def, lameq_C]);
+
+val lameq_Y = store_thm(
+  "lameq_Y",
+  ``Y @@ f == f @@ (Y @@ f)``,
+  ASSUME_TAC (Q.GEN `X` 
+                ((SIMP_CONV (betafy(srw_ss())) [lameq_S, Y_def, lameq_C] THENC 
+                  SIMP_CONV (betafy(srw_ss())) [lameq_B] THENC 
+                  SIMP_CONV (betafy(srw_ss())) [lameq_S, lameq_I, Yf1])
+                 ``Y @@ f == X``)) THEN 
+  ASM_SIMP_TAC (srw_ss()) []);
 
 val SK_incompatible = store_thm( (* example 2.18, p23 *)
   "SK_incompatible",
@@ -443,6 +469,14 @@ val bnf_Omega = Store_thm(
   "bnf_Omega",
   ``~bnf Omega``,
   SRW_TAC [][Omega_def]);
+val I_beta_normal = Store_thm(
+  "I_beta_normal",
+  ``bnf I``,
+  SRW_TAC [][I_def]);
+val K_beta_normal = Store_thm("K_beta_normal", ``bnf K``, SRW_TAC [][K_def]);
+val S_beta_normal = Store_thm("S_beta_normal", ``bnf S``, SRW_TAC [][S_def]);
+(* because I have defined them in terms of applications of S and K, C and B 
+   are not in bnf *)
 
 val bnf_vsubst_invariant = Store_thm(
   "bnf_vsubst_invariant",
@@ -518,7 +552,7 @@ val subst_eq_var = store_thm(
   Q.SPEC_THEN `t` STRUCT_CASES_TAC term_CASES THEN
   SRW_TAC [][SUB_VAR, SUB_THM] THEN PROVE_TAC []);
 
-val enf_vsubst_invariant = store_thm(
+val enf_vsubst_invariant = Store_thm(
   "enf_vsubst_invariant",
   ``!t. enf ([VAR v/u] t) = enf t``,
   HO_MATCH_MP_TAC nc_INDUCTION2 THEN
@@ -526,36 +560,15 @@ val enf_vsubst_invariant = store_thm(
   SRW_TAC [][SUB_THM, SUB_VAR, enf_thm] THEN
   SRW_TAC [boolSimps.CONJ_ss][GSYM rand_subst_commutes, subst_eq_var] THEN
   SRW_TAC [][GSYM rator_subst_commutes, FV_SUB]);
-val _ = export_rewrites ["enf_vsubst_invariant"]
-
-(*val FV_RENAMING = store_thm(
-  "FV_RENAMING",
-  ``!R. RENAMING R ==>
-        !t. FV (t ISUB R) = IMAGE (RENAME R) (FV t)``,
-  HO_MATCH_MP_TAC RENAMING_ind THEN
-  SRW_TAC [][RENAME_def, VNAME_DEF, EXTENSION, ISUB_def] THEN EQ_TAC THEN
-  SRW_TAC [][FV_SUB] THEN PROVE_TAC []);
-*)
 
 val benf_def = Define`benf t = bnf t /\ enf t`;
 
-val I_beta_normal = Store_thm(
-  "I_beta_normal",
-  ``bnf I``,
-  SRW_TAC [][I_def, bnf_thm]);
-val K_beta_normal = Store_thm(
-  "K_beta_normal",
-  ``bnf K``,
-  SRW_TAC [][K_def, bnf_thm]);
-val S_beta_normal = Store_thm(
-  "S_beta_normal",
-  ``bnf S``,
-  SRW_TAC [][S_def, bnf_thm, is_abs_thm]);
 
 val has_bnf_def = Define`has_bnf t = ?t'. t == t' /\ bnf t'`;
 
 val has_benf_def = Define`has_benf t = ?t'. t == t' /\ benf t'`;
 
+val _ = remove_ovl_mapping "Y" {Thy = "chap2", Name = "Y"}
 
 val _ = export_theory()
 end; (* struct *)
